Let $F$ be a totally ordered field and $a_1, a_2, \ldots, a_n \in F$ be positive.
Prove that
\[ \sum_{i < j} \frac{a_i a_j}{a_i + a_j} \leq \frac{n}{2(a_1 + a_2 + \ldots + a_n)} \sum_{i < j} a_i a_j. \]



\subsection*{Solution}

Official solution: \url{https://www.imo-official.org/problems/IMO2006SL.pdf}

We follow Solution 1 of the official solution with some modification.

Denote $S = a_1 + a_2 + \ldots + a_n$.
Clearly, it suffices to show that
\[ 2S \sum_{i \neq j} \frac{a_i a_j}{a_i + a_j} \leq n \sum_{i \neq j} a_i a_j. \]
Since $4 a_i a_j = (a_i + a_j)^2 - (a_i - a_j)^2$, we have
\begin{align*}
    2S \sum_{i \neq j} \frac{a_i a_j}{a_i + a_j}
    &= \frac{S}{2} \sum_{i \neq j}\left(a_i + a_j - \frac{(a_i - a_j)^2}{a_i + a_j}\right) \\
    &= (n - 1) S^2 - \frac{1}{2} \sum_{i \neq j} \frac{S (a_i - a_j)^2}{a_i + a_j} \\
    &\leq (n - 1) S^2 - \frac{1}{2} \sum_{i \neq j} (a_i - a_j)^2 \\
    &= (n - 1) S^2 - \frac{1}{2} \sum_{i, j} (a_i^2 + a_j^2 - 2 a_i a_j) \\
    &= (n - 1) S^2 - \left(n \sum_{i = 1}^n a_i^2 - S^2\right) \\
    &= nS^2 - n \sum_{i = 1}^n a_i^2 \\
    &= n \sum_{i \neq j} a_i a_j.
\end{align*}
