Determine all functions $f : \Z \to \Z$ such that
\[ f(x - f(y)) = f(f(x)) - f(y) - 1 \quad \text{for all } x, y \in \Z. \tag{*}\label{2015a2-eq0} \]



\subsection*{Answer}

$x \mapsto -1$ and $x \mapsto x + 1$.



\subsection*{Solution}

Official solution: \url{http://www.imo-official.org/problems/IMO2015SL.pdf}

We follow Solution 1 of the official solution, with some simplification in the final computation.

Plugging $x = 0$ and $y = f(0)$ into~\eqref{2015a2-eq0} gives $f(-f(f(0))) = -1$.
Then plugging $y = -f(f(0))$ into~\eqref{2015a2-eq0} gives
\[ f(x + 1) = f(f(x)) \quad \text{for all } x \in \Z. \tag{1}\label{2015a2-eq1} \]

We now prove that $f$ is linear.
That is, there exists constants $A$ and $B$ such that $f(x) = Ax + B$ for all $x \in \Z$.
For this purpose, it suffices to show that
\[ f(x + 1) = f(x) + f(-1) + 1 \quad \text{for all } x \in \Z. \]
Indeed, by~\eqref{2015a2-eq1} and~\eqref{2015a2-eq0}, for any $x \in \Z$, we have
\[ f(x + 1) - f(x) - 1 = f(f(x)) - f(x) - 1 = f(x - f(x)) + 1 = f(f(x - 1 - f(x))) + 1. \]
But by~\eqref{2015a2-eq0}, we have $f(x - 1 - f(x)) = f(x) - f(x) - 1 = -1$.
This proves that $f$ is linear.

We now finish by finding all suitable linear functions.
If $A \neq 0$, then $f$ is injective, so~\eqref{2015a2-eq1} yields $f(x) = x + 1$ for all $x \in \Z$.
Otherwise, $f$ is constant, and by plugging into~\eqref{2015a2-eq0}, we infer that this constant has to be $-1$.
That is, $f(x) = -1$ for all $x \in \Z$.
